derived_rules.v
@@ -57,7 +57,7 @@ eapply tr_sigma_intro; try assumption. simpsub. assumption.
 match goal with |- tr ?G' ?J => change J with (substj (under 0 sh1)
                                                     (deqtype b b));
                                 rewrite - 1! (cat0s G') end.
-change [::] with (@substctx False sh1 [::]).
+change [::] with (@ substctx obj sh1 [::]).
  apply tr_weakening. assumption.
 Qed.
 
@@ -74,7 +74,7 @@ Lemma tr_booltp_eta_hyp0 :
                  (subst sh1 q) )
               a).
   intros. rewrite - (cat0s ((hyp_tm booltp)::G)).
-  change (sh1) with (@under False 0 sh1).
+  change (sh1) with (@ under obj 0 sh1).
   change 0 with (size ([::]: @context False)).
   apply tr_booltp_eta_hyp; simpl; assumption.
 Qed. 
